Minimmit/Analysis/Consistency.lean
@@ -53,7 +53,7 @@ theorem own_mem_act_of_mem_succ (hinit : Init s₀) (hh : Honest f Δ lead s₀ 
 omit [DecidableEq Tx] in
 theorem localInv_init (hinit : Init s₀) (i : Fin n) : Algo.LocalInv f i (s₀.procs i) := by
   rw [hinit.procs i]
-  refine ⟨⟨le_refl 1, ?_, ?_, ?_, ?_, ?_, ?_⟩, ?_⟩ <;> simp [Processor.init]
+  refine ⟨⟨le_refl 1, ?_, ?_, ?_, ?_, ?_, ?_⟩, ?_, ?_⟩ <;> simp [Processor.init]
 
 theorem localInv_step (hinit : Init s₀) (hh : Honest f Δ lead s₀ instrs) {i : Fin n}
     (hi : Correct s₀ instrs i) (t : Nat) (h : Algo.LocalInv f i ((State.run s₀ instrs t).procs i)) :
